added comments

ModelTheory.v
@@ -6,9 +6,16 @@ Notation "x :: l" := (cons x l) (at level 60, right associativity).
 Notation "[ ]" := nil.
 Notation "[ x ; .. ; y ]" := (cons x .. (cons y nil) ..).
 
+(* Here I have formalized the basic definitions of model theory in Coq and proved some basic theorems 
+I have followed this text: http://www.math.toronto.edu/weiss/model_theory.pdf. *)
+
 (******************************************************************************************)
 (* Args *)
 (******************************************************************************************)
+
+(* Argument tuples are lists parameterized by length. These types are passed to functions
+and relations. Specifically an n-place function will take an n-tuple args as its parameter
+and an m-place relation will take an m-typle args as its parameter.*)
 
 (* Inductive type idea and notation taken from
  http://www.cs.cornell.edu/courses/cs6115/2017fa/notes/lecture8.html *)
@@ -23,26 +30,41 @@ Local Notation "[| x ; .. ; y |]" := (@consA _ _ x (.. (@consA _ _ y (@nilA _)) 
 (* Symbols *)
 (******************************************************************************************)
 
+(* In model theory there are symbols for variables, functions, constants, and relations, along with
+all the usual logic connectives and quantifiers, which we will see later in the formula section. *)
+
 Inductive var : Type :=
-| Var : nat -> var.
+(* The nat is the variable identifier. *)
+| Var : nat -> var. 
 Inductive func : Type :=
-| Func : nat -> nat -> func.
+(* The first nat is the function identifier and the second nat is the function arity. *)
+| Func : nat -> nat -> func. 
 Inductive const : Type :=
+(* The first nat is the constant identifier. *)
 | Const : nat -> const.
 Inductive rel : Type :=
+(* The first nat is the relation identifier and the second nat is the relation arity. *)
 | Rel : nat -> nat -> rel.
 
 (******************************************************************************************)
 (* Terms *)
 (******************************************************************************************)
 
+(* Terms in model theory are variables, constants, or n-place functions which take n arguments, 
+all of which are also terms. *)
+
+(* Does the arity of the function f match arity? *)
 Definition arity_match_func (f : func) (arity : nat) := match f with
 | Func _ ar => arity = ar
 end.
 
 Inductive term : Type :=
+(* Wraps a variable symbol. *)
 | VarT   : var -> term
+(* Wraps a constant symbol. *)
 | ConstT : const -> term
+(* Function terms consist of a symbol, an arity, a term argument tuple of that arity, 
+and a proof that the symbol arity matches the specified arity. *)
 | FuncT  : forall (f : func) (arity : nat) (arg : args term arity), 
             (arity_match_func f arity) -> term.
 
@@ -58,16 +80,26 @@ End func_inst_example.
 (* Formulas *)
 (******************************************************************************************)
 
+(* Formulas in model theory are relations (including the special equals relation, which is a 
+part of any language), as well as the usual logical connectives applied to formulas. Note that
+Equals and Relates formulas are known as atomic formulas. *)
+
 Definition arity_match_rel (r : rel) (arity : nat) := match r with
 | Rel _ ar => arity = ar
 end.
 
-Inductive formula : Type := 
+Inductive formula : Type :=
+(* Equals formulas takes in two formulas and always as the usual interpretation of equality. *) 
 | Equals  : term -> term -> formula
+(* Relates formulas consist of a symbol, an arity, a term argument tuple of that arity
+and a proof that the symbol arity matches the specified arity. *)
 | Relates : forall (r : rel) (arity : nat) (arg : args term arity), 
             (arity_match_rel r arity) -> formula
+(* Usual logical Not. *)
 | Not     : formula -> formula
+(* Usual logical Or. *)
 | Or      : formula -> formula -> formula
+(* Usual predicate calculus quantification. *)
 | Forall  : var -> formula -> formula.
 
 (* Derived formulas *)
@@ -80,13 +112,22 @@ Definition Exists (v : var) (phi : formula) := Not (Forall v (Not phi)).
 (* Subformulas *)
 (******************************************************************************************)
 
+(* Here we define the notion of a subformula of a formula. *)
 Inductive subformula : formula -> formula -> Prop :=
 | SubIden   (psi phi : formula) : psi = phi -> subformula psi phi
+(* If psi is the same as phi, psi is a subformula of phi. *)
 | SubNot    (psi phi : formula) : subformula (Not psi) phi -> subformula psi phi
+(* If Not psi is a subformula of phi, psi is a subformula of phi. *)
 | SubOrL    (theta psi phi : formula) : subformula (Or theta psi) phi -> subformula theta phi
+(* If Or theta psi is a subformula of phi, theta is a subformula of phi. *)
 | SubOrR    (theta psi phi : formula) : subformula (Or theta psi) phi -> subformula psi phi
+(* If Or theta psi is a subformula of phi, psi is a subformula of phi. *)
 | SubForall (v : var) (psi phi : formula) : subformula (Forall v psi) phi -> subformula psi phi.
+(* If Forall v psi is a subformula of phi, psi is a subformula of phi. *)
 
+(* Below are proofs about subformulas for derived formulas. *)
+
+(* If And theta psi is a subformula of phi, theta is a subformula of phi. *)
 Theorem SubAndL : forall (theta psi phi : formula), 
   subformula (And theta psi) phi -> subformula theta phi.
 Proof.
@@ -98,6 +139,7 @@ Proof.
   assumption.
 Qed.
 
+(* If And theta psi is a subformula of phi, psi is a subformula of phi. *)
 Theorem SubAndR : forall (theta psi phi : formula),
   subformula (And theta psi) phi -> subformula psi phi.
 Proof.
@@ -109,6 +151,7 @@ Proof.
   assumption.
 Qed.
 
+(* If Impl theta psi is a subformula of phi, theta is a subformula of phi. *)
 Theorem SubImplL : forall (theta psi phi : formula),
   subformula (Impl theta psi) phi -> subformula theta phi.
 Proof.
@@ -119,6 +162,7 @@ Proof.
   assumption.
 Qed.
 
+(* If Impl theta psi is a subformula of phi, psi is a subformula of phi. *)
 Theorem SubImplR : forall (theta psi phi : formula),
   subformula (Impl theta psi) phi -> subformula psi phi.
 Proof.
@@ -128,6 +172,7 @@ Proof.
   assumption.
 Qed.
 
+(* If Iff theta psi is a subformula of phi, theta is a subformula of phi. *)
 Theorem SubIffL : forall (theta psi phi : formula),
   subformula (Iff theta psi) phi -> subformula theta phi.
 Proof.
@@ -138,6 +183,7 @@ Proof.
   assumption.
 Qed.
 
+(* If Iff theta psi is a subformula of phi, psi is a subformula of phi. *)
 Theorem SubIffR : forall (theta psi phi : formula),
   subformula (Iff theta psi) phi -> subformula psi phi.
 Proof.
@@ -148,6 +194,7 @@ Proof.
   assumption.
 Qed.
 
+(* If Exists v psi is a subformula of phi, psi is a subformula of phi. *)
 Theorem SubExists : forall (v : var) (psi phi : formula),
   subformula (Exists v psi) phi -> subformula psi phi.
 Proof.
@@ -208,11 +255,17 @@ end.
 (* Free variables *)
 (******************************************************************************************)
 
+(* Given a formula, a variable is in the set of that formula's free variables if and only if
+it appears outside the syntatic scope of a quantifier at least once in that formula. *)
+
+(* Helper type that represents function arguments as a list rather than an args. 
+This is so we can use the useful list functions rather than deal with cumbersome arg terms. *)
 Inductive termList : Type :=
 | VarTList   : var -> termList
 | ConstTList : const -> termList
 | FuncTList  : func -> (list termList ) -> termList.
 
+(* Converts a term to a termList. *)
 Fixpoint term_to_termlist (t : term) := 
 
 let _args_to_list := (fix _args_to_list (n : nat) (a : args term n) := match a with
@@ -226,14 +279,17 @@ match t with
 | FuncT f n a _ => FuncTList f (_args_to_list n a) 
 end.
 
+(* Returns a list of all the variables mentioned in the termList. *)
 Fixpoint term_vars_helper (t : termList) := match t with
 | VarTList v    => v::[]
 | ConstTList c  => []
 | FuncTList f l => fold_left (fun acc x => acc++(term_vars_helper x)) l []
 end.
 
+(* Returns a list of all the variables mentioned in the term. *)
 Definition term_vars (t : term) := term_vars_helper (term_to_termlist t).
 
+(* Converts an args term n into a list term. *)
 Fixpoint args_to_list (n : nat) (a : args term n) := match a with
 | nilA _ => []
 | consA _ n' h t' => (term_to_termlist h)::(args_to_list n' t')
@@ -246,6 +302,7 @@ Definition tv := term_vars t.
 Theorem thm : contains_var tv (Var 1) = true. Proof. reflexivity. Qed.
 End term_vars_example.
 
+(* Returns the free variables of phi. *)
 Fixpoint free_vars (phi : formula) := match phi with 
 | Equals t1 t2      => (term_vars t1)++(term_vars t2)
 | Relates r n a _   => fold_left (fun a x => a++(term_vars_helper x)) (args_to_list n a) []
@@ -269,18 +326,15 @@ End free_vars_example.
 (* Substitution *)
 (******************************************************************************************)
 
-Definition x := [|1; 2; 3|].
-Check x.
+(* Given a formula phi, a variable v, and a term t, define substitution to be syntactic replacement
+of all free occurrences of v with t in phi. *)
 
-Definition x' := consA nat 3 1 x.
-Check x.
-
+(* Term substitution. Substitutes all occurrences of v with t in t_orig. *)
 Fixpoint subst_term (t_orig : term) (v : var) (t : term) := 
 let subst_term_args := (fix subst_term_args (n : nat) (a : args term n) := match a with
 | nilA _ => nilA _ 
 | consA _ n' h t' => consA _ n' (subst_term h v t) (subst_term_args n' t')
-end
-) in
+end) in
 
 match t_orig with
 | VarT v    => t
@@ -292,8 +346,7 @@ Fixpoint subst_helper (phi: formula) (v : var) (t : term) (free : list var) :=
 let subst_term_args := (fix subst_term_args (n : nat) (a : args term n) := match a with
 | nilA _ => nilA _
 | consA _ n' h t' => consA  _ n' (subst_term h v t) (subst_term_args n' t')
-end
-) in
+end) in
 
 match phi with
 | Equals t1 t2    =>  if (contains_var free v) then 
@@ -309,6 +362,7 @@ match phi with
 | Forall v' psi   => Forall v' (subst_helper psi v t (remove_var free v'))
 end.
 
+(* Formula substitution. Substitutes all free occurrences of v with t in phi. *)
 Definition subst (phi: formula) (v : var) (t : term) := subst_helper phi v t (free_vars phi).
 
 Module subst_example.
@@ -327,32 +381,42 @@ End subst_example.
 (* Languages *)
 (******************************************************************************************)
 
+(* A language in model theory is defined as a set of constant, relation, and function symbols.*)
 Inductive lang : Type :=
 | Lang : list const -> list rel -> list func -> lang.
-
 Definition lang_const (l : lang) := match l with
 | Lang c r f => c
 end.
-
 Definition lang_rel (l : lang) := match l with
 | Lang c r f => r
 end.
-
 Definition lang_func (l : lang) := match l with
 | Lang c r f => f
 end.
 
-Fixpoint valid_term (language : lang) (t : term) := match t with
-| VarT _    => true
-| ConstT c  => contains_const (lang_const language) c
-| FuncT f l => contains_func (lang_func language) f && 
-              (fold_left (fun a x => (valid_term language x) && a) l true)
+(* A term is valid with respect to a language if it only mentions symbols from that language. *)
+Fixpoint valid_term (language : lang) (t : term) := 
+let valid_term_args := (fix valid_term_args (n : nat) (a : args term n) := match a with
+| nilA _ => true
+| consA _ n' h t => (valid_term language h) && (valid_term_args n' t)
+end) in
+
+match t with
+| VarT _        => true
+| ConstT c      => contains_const (lang_const language) c
+| FuncT f n a _ => contains_func (lang_func language) f && (valid_term_args n a)
 end.
 
-Fixpoint valid_formula (language : lang) (phi : formula) := match phi with
+(* A formula is valid with respect to a language if it only mentions symbols from that language. *)
+Fixpoint valid_formula (language : lang) (phi : formula) := 
+let valid_term_args := (fix valid_term_args (n : nat) (a : args term n) := match a with
+| nilA _ => true
+| consA _ n' h t => (valid_term language h) && (valid_term_args n' t)
+end) in
+
+match phi with
 | Equals t1 t2  => (valid_term language t1) && (valid_term language t2)
-| Relates r l   => contains_rel (lang_rel language) r &&
-                   (fold_left (fun a x => (valid_term language x) && a) l true)
+| Relates r n a _ => contains_rel (lang_rel language) r && (valid_term_args n a)
 | Not psi       => valid_formula language psi
 | Or psi theta  => (valid_formula language psi) && (valid_formula language theta)
 | Forall _ psi  => valid_formula language psi
@@ -363,11 +427,12 @@ Definition c1 := ConstT (Const 1).
 Definition c2 := ConstT (Const 2).
 Definition c3 := ConstT (Const 3).
 Definition v1 := Var 1.
-Definition r1 := (Rel 1 (Arity 2)).
-Definition phi := Or (Equals c1 c2) (Forall v1 (Relates r1 [VarT v1; c3])).
-Definition l := Lang [Const 1; Const 2; Const 3]  [Rel 1 (Arity 2)] [].
+Definition r1 := (Rel 1 2).
+Theorem am : arity_match_rel r1 2. Proof. reflexivity. Qed.
+Definition phi := Or (Equals c1 c2) (Forall v1 (Relates r1 2 [|VarT v1; c3|] am)).
+Definition l := Lang [Const 1; Const 2; Const 3]  [Rel 1 2] [].
 Theorem thm1 : (valid_formula l phi) = true. Proof. reflexivity. Qed.
-Definition l' := Lang [Const 1; Const 2] [Rel 1 (Arity 2)] [].
+Definition l' := Lang [Const 1; Const 2] [Rel 1 2] [].
 Theorem thm2: (valid_formula l' phi) = false. Proof. reflexivity. Qed.
 End valid_formula_example.
 
@@ -375,34 +440,46 @@ End valid_formula_example.
 (* Models *)
 (******************************************************************************************)
 
+(* Given a language L, a model is a tuple (A, I) where A is a set (called the universe of the model)
+and I is an interpretation function for the constant, function, and relation symbols for L. 
+If a symbol F is an n-place function symbol, then I(F) is an n-place function
+symbol on A. If a symbol R is an m-place relation symbol, then I(R) is an m-place relation
+symbol on A. If a symbol C is a constant symbol, then I(C) is an element of A. Note that constants
+can be viewed as a degenerate case of functions, namely a function that takes 0 arguments.*)
+
 (* Note that it isn't strictly necesary to tie interpretation functions to a language, since
 interpretation functions for constants/functions/relations can simply map all symbols 
 not in a given language to a single value. For example, if a language has constants
 {Const 1, Const 2}, an interpretation function can map Const 1 to v1, Const 2 to v2, 
 and all other constants to v1. Similar reasoning applies to functions and relations. *)
 
-(* FixMe: how to deal with function/relation airities? *)
-(* FixMe: how to tie interp functions to lang? *)
-
+(* The constant portion of the symbol interpretation function maps each constant symbol to an element of A. *)
 Inductive constInterp (A : Type) : Type :=
 | ConstInterp : (const -> A) -> constInterp A.
 
+(* The function portion of the symbol interpretation function maps each n-place function symbol 
+to a n-place function on A. *)
 Inductive funcInterp (A : Type) : Type :=
 | FuncInterp : (func -> (list A) -> A) -> funcInterp A.
 
+(* The relation portion of the symbol interpretation function maps each m-place relation symbol
+to an m-place relation on A. *)
 Inductive relInterp (A : Type) : Type :=
 | RelInterp : (rel -> (list A) -> Prop) -> relInterp A.
 
+(* The symbol interpretation function is a composite of the constant, function, and relation
+symbol interpretation functions. *)
 Inductive interpretation (A : Type) : Type :=
 | Interpretation : (constInterp A) -> (funcInterp A) -> (relInterp A) -> interpretation A.
 
+(* A model is a composite of a language and an interpretation function. *)
 Inductive model (A : Type) : Type := 
 | Model : lang -> (interpretation A) -> model A.
 
 Module model_example.
 Definition zero := Const 0.
-Definition plus := Func 0 2).
-Definition times := Func 1 2).
+Definition plus := Func 0 2.
+Definition times := Func 1 2.
 Definition simpleLang := Lang [zero] [] [plus].
 Definition cInterp (c : const) := if eq_const c zero then 0 else 0.
 Fixpoint fInterp (f : func) (args : list nat) :=
